Simplify history wrappper and store increasing_map in NA points-to predicate

src/high/dprop.v
@@ -2,7 +2,7 @@
 logic. *)
 
 From iris.bi Require Export monpred.
-From iris.proofmode Require Import monpred.
+From iris.proofmode Require Import monpred tactics.
 From iris.base_logic.lib Require Import iprop.
 
 From self Require Export view memory.
@@ -27,7 +27,44 @@ Definition dProp Σ := monPred thread_view_bi_index (iPropI Σ).
 Definition dPropO Σ := monPredO thread_view_bi_index (iPropI Σ).
 Definition dPropI Σ := monPredI thread_view_bi_index (iPropI Σ).
 
+Ltac iModel := iStartProof (iProp _); iIntros (TV).
+
 (* [bi_scope] is the scope associated with the scope key [I] from Iris. We bind
 it to the [dProp] type such that we avoid having to type `%I` to get the right
 scope when writing definitions of type [dProp]. *)
 Bind Scope bi_scope with dProp.
+
+Section definitions.
+  Context {Σ : gFunctors}.
+
+  Program Definition have_SV ℓ t : dProp Σ :=
+    MonPred (λ TV, ⌜ t ≤ (store_view TV) !!0 ℓ ⌝)%I _.
+  Next Obligation. solve_proper. Qed.
+
+  Global Instance have_SV_persistent ℓ t : Persistent (have_SV ℓ t).
+  Proof. apply monPred_persistent=> j. apply _. Qed.
+
+  Program Definition have_FV ℓ t : dProp Σ :=
+    MonPred (λ TV, ⌜ t ≤ (flush_view TV) !!0 ℓ ⌝)%I _.
+  Next Obligation. solve_proper. Qed.
+
+  Global Instance have_FV_persistent ℓ t : Persistent (have_FV ℓ t).
+  Proof. apply monPred_persistent=> j. apply _. Qed.
+
+  Lemma have_SV_0 ℓ : ⊢ have_SV ℓ 0.
+  Proof. iModel. iPureIntro. lia. Qed.
+
+  Lemma have_FV_0 ℓ : ⊢ have_FV ℓ 0.
+  Proof. iModel. iPureIntro. lia. Qed.
+
+  Lemma monPred_in_have_SV SV PV BV ℓ t :
+    t ≤ SV !!0 ℓ →
+    monPred_in (SV, PV, BV) -∗
+    have_SV ℓ t.
+  Proof.
+    intros le.
+    iStartProof (iProp _). iPureIntro. intros [[SV' ?] ?] [[incl ?]?].
+    etrans; first done. f_equiv. done.
+  Qed.
+
+ End definitions.
