src/high/resources/abstract_history.v
@@ -1,4 +1,5 @@
-(* Resource algebra to represent abstract histories. *)
+(* Ghost state to represent abstract histories. This is just a few extra
+definitions and lemmas on top of [ghost_map_map]. *)
 
 From iris.bi Require Import lib.fractional.
 From iris.algebra Require Import auth gmap.
@@ -9,44 +10,22 @@ From iris.proofmode Require Import proofmode.
 From self.algebra Require Import ghost_map ghost_map_map.
 From self.lang Require Import lang.
 From self Require Import extra.
-(* From self.high.resources Require Import auth_map_map. *)
 
 (* For abstract history we need two types of fragmental knowledge. One that
 represents ownership about the entire abstract history of a location (for
 non-atomic) and one that represents only knowledge about one entry in the
 abstract history. *)
 
-(* Resource algebras that for each location stores the encoded abstract states
-associated with each message/store. *)
-(* Definition encoded_abs_historyR := gmapUR time (agreeR positiveO). *)
-
-(* Definition know_abs_historiesR := auth_map_mapR positiveO. *)
-
 (** We define a few things about the resource algebra that that we use to encode
 abstract histories. *)
 Section abs_history_lemmas.
   Context `{ghost_map_mapG Σ loc time positive}.
-  (* Context `{!ghost_mapG Σ loc (gmap time positive), inG Σ know_abs_historiesR}. *)
   Context `{Countable ST}.
 
   Implicit Types
     (abs_hist : gmap time ST) (ℓ : loc)
     (enc_abs_hist : gmap time positive)
     (abs_hists : gmap loc (gmap time positive)).
-
-  (* Definition abs_hist_to_ra abs_hist : encoded_abs_historyR := *)
-  (*   (to_agree ∘ encode) <$> abs_hist. *)
-
-  (* If we own the full history then we own the authorative view of both the
-  resource algebras. *)
-  Definition history_full_map γ abs_hists : iProp Σ :=
-    full_map γ (DfracOwn 1) abs_hists.
-
-  Definition history_frag_entry γ ℓ t e : iProp Σ :=
-    frag_entry γ ℓ t e.
-
-  (* Definition history_frag_entry γ ℓ enc_abs_hist : iProp Σ := *)
-  (*   full_entry γ ℓ enc_abs_hist. *)
 
   (* In this definition we store that decoding the stored encoded histry is
   equal to our abstract history. This is weaker than strogin the other way
@@ -56,190 +35,37 @@ Section abs_history_lemmas.
   return [store_lb] for the returned state. At that point we can conclude that
   decoding the encoding gives a result but not that the encoding is an encoding
   of some state. *)
-  Definition history_frag_entry_unenc γ ℓ t (s : ST) : iProp Σ :=
-    ∃ e, ⌜ decode e = Some s ⌝ ∗ history_frag_entry γ ℓ t e.
+  Definition frag_entry_unenc γ ℓ t (s : ST) : iProp Σ :=
+    ∃ e, ⌜ decode e = Some s ⌝ ∗ frag_entry γ ℓ t e.
 
   Definition history_full_entry_encoded γ ℓ q enc_abs_hist : iProp Σ :=
     full_entry γ ℓ (DfracOwn q) enc_abs_hist.
-    (* ℓ ↪[ γ ]{#q} enc_abs_hist ∗ *)
-    (* history_frag_entry ℓ enc_abs_hist. *)
 
-  Definition history_full_map_loc γ ℓ q abs_hist : iProp Σ :=
-    history_full_entry_encoded γ ℓ q (encode <$> abs_hist).
+  Definition full_entry_unenc γ ℓ q abs_hist : iProp Σ :=
+    full_entry γ ℓ (DfracOwn q) (encode <$> abs_hist).
 
-  (* Global Instance own_full_encoded_history_fractional γ ℓ enc_abs_hist : *)
-  (*   Fractional (λ q, history_full_entry_encoded γ ℓ q enc_abs_hist). *)
-  (* Proof. apply _. *)
-  (*   intros p q. *)
-  (*   rewrite /history_full_entry_encoded. *)
-  (*   iSplit. *)
-  (*   - iIntros "[[$$] #?]". iFrame "#". *)
-  (*   - iIntros "[[$ $] [$ _]]". *)
-  (* Qed. *)
-  (* Global Instance own_full_encoded_history_as_fractional γ ℓ q enc_abs_hist : *)
-  (*   AsFractional *)
-  (*     (history_full_entry_encoded γ ℓ q enc_abs_hist) *)
-  (*     (λ q, history_full_entry_encoded γ ℓ q enc_abs_hist)%I q. *)
-  (* Proof. split; [done | apply _]. Qed. *)
-
-  Lemma history_full_map_loc_agree γ ℓ q p abs_hist1 abs_hist2 :
-    history_full_map_loc γ ℓ q abs_hist1 -∗
-    history_full_map_loc γ ℓ p abs_hist2 -∗
+  Lemma full_entry_unenc_agree γ ℓ q p abs_hist1 abs_hist2 :
+    full_entry_unenc γ ℓ q abs_hist1 -∗
+    full_entry_unenc γ ℓ p abs_hist2 -∗
     ⌜ abs_hist1 = abs_hist2 ⌝.
   Proof.
     iIntros "[A _]". iIntros "[B _]".
     iDestruct (full_entry_agree with "A B") as %<-%(inj _). done.
   Qed.
 
-  (* Lemma history_full_map_loc_to_frag γ ℓ q abs_hist : *)
-  (*   history_full_map_loc γ ℓ q abs_hist -∗ *)
-  (*   history_frag_entry_unenc γ ℓ abs_hist. *)
-  (* Proof. *)
-  (*   iIntros "[_ H]". iExists _. iFrame "H". *)
-  (*   iPureIntro. *)
-  (*   apply map_eq. intros t. *)
-  (*   rewrite 3!lookup_fmap. *)
-  (*   destruct (abs_hist !! t); last done. *)
-  (*   simpl. rewrite decode_encode. done. *)
-  (* Qed. *)
-
-  (* Lemma history_frag_entry_unenc_lookup ℓ abs_hist t h : *)
-  (*   abs_hist !! t = Some h → *)
-  (*   history_frag_entry_unenc ℓ abs_hist -∗ *)
-  (*   history_frag_entry_unenc ℓ {[ t := h ]}. *)
-  (* Proof. *)
-  (*   iIntros (look). *)
-  (*   iIntros "(%m & %eq & H)". *)
-  (*   setoid_rewrite map_eq_iff in eq. *)
-  (*   specialize (eq t). *)
-  (*   rewrite 2!lookup_fmap in eq. *)
-  (*   rewrite look in eq. *)
-  (*   simpl in eq. *)
-  (*   rewrite -lookup_fmap in eq. *)
-  (*   apply lookup_fmap_Some in eq as (e & dec & mLook). *)
-  (*   iExists ({[ t := e ]}). *)
-  (*   iDestruct (auth_map_map_frag_lookup_singleton with "H") as "$". *)
-  (*   { rewrite lookup_singleton. done. } *)
-  (*   { done. } *)
-  (*   iPureIntro. *)
-  (*   rewrite !map_fmap_singleton. *)
-  (*   congruence. *)
-  (* Qed. *)
-
-  (* Lemma history_full_map_alloc h : *)
-  (*   ⊢ |==> ∃ γ , *)
-  (*     history_full_map γ h ∗ *)
-  (*     (* auth_map_map_frag h ∗ *) *)
-  (*     ([∗ map] k↦v ∈ h, *)
-  (*       history_full_entry_encoded γ k 1 v ∗ *)
-  (*       ([∗ map] k2 ↦ x ∈ v, history_frag_entry γ k k2 x)). *)
-  (* Proof. *)
-  (*   apply full_map_alloc. *)
-  (*   (* iMod (ghost_map_alloc h) as (new_abs_history_name) "[A B]". *) *)
-  (*   (* iExists _. iFrame "A B". *) *)
-  (*   (* setoid_rewrite <- own_op. *) *)
-  (*   (* iMod (own_alloc _) as "$". *) *)
-  (*   (* { apply auth_both_valid_2; last reflexivity. *) *)
-  (*   (*   intros k. *) *)
-  (*   (*   rewrite lookup_fmap. *) *)
-  (*   (*   case (h !! k); simpl; last done. *) *)
-  (*   (*   intros ? k'. *) *)
-  (*   (*   apply Some_valid. *) *)
-  (*   (*   rewrite lookup_fmap. *) *)
-  (*   (*   case (g !! k'); done. } *) *)
-  (*   (* done. *) *)
-  (* Qed. *)
-
   Lemma own_full_equiv γ ℓ q abs_hist :
-    history_full_map_loc γ ℓ q abs_hist ⊣⊢
+    full_entry_unenc γ ℓ q abs_hist ⊣⊢
       history_full_entry_encoded γ ℓ q (encode <$> abs_hist).
   Proof. done. Qed.
 
   Lemma frag_history_equiv γ ℓ t s :
     frag_entry γ ℓ t (encode s) -∗
-    history_frag_entry_unenc γ ℓ t s.
+    frag_entry_unenc γ ℓ t s.
   Proof. iIntros "H". iExists _. iFrame. rewrite decode_encode. done. Qed.
 
-  (* Lemma own_frag_equiv γ ℓ abs_hist : *)
-  (*   history_frag_entry γ ℓ (encode <$> abs_hist) ⊢ *)
-  (*   history_frag_entry_unenc γ ℓ abs_hist. *)
-  (* Proof. *)
-  (*   rewrite /history_frag_entry_unenc /history_frag_entry. *)
-  (*   iIntros "H". *)
-  (*   iExists _. iFrame. iPureIntro. *)
-  (*   apply map_eq. intros t. *)
-  (*   rewrite !lookup_fmap. *)
-  (*   destruct (abs_hist !! t); last done. *)
-  (*   simpl. by rewrite decode_encode. *)
-  (* Qed. *)
-
-  (* Lemma abs_hist_to_ra_inj hist hist' : *)
-  (*   abs_hist_to_ra hist' ≡ abs_hist_to_ra hist → *)
-  (*   hist' = hist. *)
-  (* Proof. *)
-  (*   intros eq. *)
-  (*   apply: map_eq. intros t. *)
-  (*   pose proof (eq t) as eq'. *)
-  (*   rewrite !lookup_fmap in eq'. *)
-  (*   destruct (hist' !! t) as [h|] eqn:leq, (hist !! t) as [h'|] eqn:leq'; *)
-  (*     try inversion eq'; auto. *)
-  (*   simpl in eq'. *)
-  (*   apply Some_equiv_inj in eq'. *)
-  (*   apply to_agree_inj in eq'. *)
-  (*   apply encode_inj in eq'. *)
-  (*   rewrite eq'. *)
-  (*   done. *)
-  (* Qed. *)
-
-  (* Lemma abs_hist_to_ra_agree hist hist' : *)
-  (*   to_agree <$> hist' ≡ abs_hist_to_ra hist → hist' = encode <$> hist. *)
-  (* Proof. *)
-  (*   intros eq. *)
-  (*   apply: map_eq. intros t. *)
-  (*   pose proof (eq t) as eq'. *)
-  (*   rewrite !lookup_fmap in eq'. *)
-  (*   rewrite lookup_fmap. *)
-  (*   destruct (hist' !! t) as [h|] eqn:leq, (hist !! t) as [h'|] eqn:leq'; *)
-  (*     try inversion eq'; auto. *)
-  (*   simpl in eq'. simpl. *)
-  (*   apply Some_equiv_inj in eq'. *)
-  (*   apply to_agree_inj in eq'. *)
-  (*   f_equiv. *)
-  (*   apply eq'. *)
-  (* Qed. *)
-
-  (** If you know the full history for a location and own the "all-knowing"
-  resource, then those two will agree. *)
-  Lemma history_full_map_agree γ ℓ q hist hists :
-    history_full_map γ hists -∗
-    history_full_map_loc γ ℓ q hist -∗
-    ⌜hists !! ℓ = Some (encode <$> hist)⌝.
-  Proof.
-    iIntros "A [B _]".
-    iApply (full_map_full_entry with "A B").
-  Qed.
-
-  (* Lemma own_frag_history_agree γ ℓ (part_hist : gmap time ST) hists : *)
-  (*   history_full_map γ hists -∗ *)
-  (*   history_frag_entry_unenc ℓ part_hist -∗ *)
-  (*   ⌜∃ hist, hists !! ℓ = Some (hist) ∧ *)
-  (*           (Some <$> part_hist) ⊆ (decode <$> hist)⌝. *)
-  (* Proof. *)
-  (*   rewrite /history_full_map. *)
-  (*   iIntros "[O A]". *)
-  (*   iDestruct 1 as (enc) "[%eq K]". *)
-  (*   iDestruct (own_valid_2 with "A K") as %[incl _]%auth_both_valid_discrete. *)
-  (*   apply fmap_fmap_to_agree_singleton_included_l in incl. *)
-  (*   destruct incl as [hist' [look incl]]. *)
-  (*   iPureIntro. *)
-  (*   exists hist'. *)
-  (*   split. { apply leibniz_equiv. done. } *)
-  (*   rewrite -eq. apply map_fmap_mono. done. *)
-  (* Qed. *)
-
-  Lemma history_full_map_frag_singleton_agreee γ ℓ t (s : ST) hists :
-    history_full_map γ hists -∗
-    history_frag_entry_unenc γ ℓ t s -∗
+  Lemma full_map_frag_singleton_agreee γ dq ℓ t (s : ST) hists :
+    full_map γ dq hists -∗
+    frag_entry_unenc γ ℓ t s -∗
     ⌜∃ hist enc,
       hists !! ℓ = Some hist ∧ hist !! t = Some enc ∧ decode enc = Some s⌝.
   Proof.
@@ -248,23 +74,9 @@ Section abs_history_lemmas.
     iPureIntro. eexists _, _. split_and!; done.
   Qed.
 
-  (* Lemma history_full_map_lookup γ abs_hists enc_abs_hist ℓ t s : *)
-  (*   abs_hists !! ℓ = Some enc_abs_hist → *)
-  (*   enc_abs_hist !! t = Some s → *)
-  (*   history_full_map γ abs_hists ==∗ *)
-  (*   history_full_map γ abs_hists ∗ *)
-  (*   history_frag_entry γ ℓ t s. *)
-  (* Proof. *)
-  (*   iIntros (look1 look2). *)
-  (*   iIntros "[M N]". *)
-  (*   iMod (auth_map_map_lookup with "N") as "[N hip]"; try done. *)
-  (*   iFrame. *)
-  (*   done. *)
-  (* Qed. *)
-
   Lemma own_frag_history_singleton_agreee γ ℓ t s1 s2 :
-    history_frag_entry_unenc γ ℓ t s1 -∗
-    history_frag_entry_unenc γ ℓ t s2 -∗
+    frag_entry_unenc γ ℓ t s1 -∗
+    frag_entry_unenc γ ℓ t s2 -∗
     ⌜ s1 = s2 ⌝.
   Proof.
     iDestruct 1 as (enc deq) "K".
@@ -272,64 +84,5 @@ Section abs_history_lemmas.
     iDestruct (frag_entry_agree with "K K'") as %<-.
     iPureIntro. congruence.
   Qed.
-
-  (* Lemma history_full_map_alloc_frag γ ℓ t encS (s : ST) hists hist : *)
-  (*   hists !! ℓ = Some hist → *)
-  (*   hist !! t = Some encS → *)
-  (*   decode encS = Some s → *)
-  (*   history_full_map γ hists ==∗ *)
-  (*   history_full_map γ hists ∗ history_frag_entry_unenc γ ℓ {[ t := s ]}. *)
-  (* Proof. *)
-  (*   iIntros (look lookHist decEq) "M". *)
-  (*   iMod (history_full_map_lookup with "M") as "[M hi]"; try done. *)
-  (*   iFrame. iModIntro. *)
-  (*   rewrite /history_frag_entry_unenc. *)
-  (*   iExists {[ t := encS ]}. *)
-  (*   rewrite /history_frag_entry. *)
-  (*   rewrite !map_fmap_singleton. *)
-  (*   rewrite decEq. *)
-  (*   iFrame. *)
-  (*   done. *)
-  (* Qed. *)
-
-  (* Insert a new location into an abstract history. *)
-  (* Lemma history_full_map_history_insert_loc γ abs_hists ℓ enc_abs_hist : *)
-  (*   abs_hists !! ℓ = None → *)
-  (*   history_full_map γ abs_hists ==∗ *)
-  (*   history_full_map γ (<[ℓ := enc_abs_hist]>abs_hists) ∗ *)
-  (*   history_full_entry_encoded γ ℓ 1 enc_abs_hist. *)
-  (*   (* history_frag_entry γ ℓ enc_abs_hist. *) *)
-  (* Proof. apply full_map_insert. Qed. *)
-
-  (* Insert a new message into an abstract history. *)
-  (* Lemma own_full_encoded_history_insert γ ℓ t enc_abs_hist abs_hists encS : *)
-  (*   enc_abs_hist !! t = None → *)
-  (*   history_full_map γ abs_hists -∗ *)
-  (*   history_full_entry_encoded γ ℓ 1 enc_abs_hist ==∗ *)
-  (*   let enc_abs_hist' := <[t := encS]>enc_abs_hist *)
-  (*   in history_full_map γ (<[ℓ := enc_abs_hist']>abs_hists) ∗ *)
-  (*      history_full_entry_encoded γ ℓ 1 enc_abs_hist' ∗ *)
-  (*      history_frag_entry γ ℓ t encS. *)
-  (* Proof. apply full_map_full_entry_insert. Qed. *)
-
-  (* Insert a new message into an abstract history. *)
-  (* Lemma history_full_map_insert γ ℓ t abs_hist abs_hists (s : ST) : *)
-  (*   abs_hist !! t = None → *)
-  (*   history_full_map γ abs_hists -∗ *)
-  (*   history_full_map_loc γ ℓ 1 abs_hist ==∗ *)
-  (*   let abs_hist' := <[t := s]>abs_hist *)
-  (*   in history_full_map γ (<[ℓ := encode <$> abs_hist']>abs_hists) ∗ *)
-  (*      history_full_map_loc γ ℓ 1 abs_hist' ∗ *)
-  (*      history_frag_entry_unenc γ ℓ t s. *)
-  (* Proof. *)
-  (*   iIntros (look) "??". *)
-  (*   iMod (own_full_encoded_history_insert with "[$] [$]") as "(H1 & H2 & H3)". *)
-  (*   { rewrite lookup_fmap. apply fmap_None. done. } *)
-  (*   iModIntro. *)
-  (*   rewrite /history_full_map_loc /history_frag_entry_unenc fmap_insert. *)
-  (*   iFrame "H1 H2". *)
-  (*   iExists _. iFrame. *)
-  (*   iPureIntro. rewrite decode_encode. done. *)
-  (* Qed. *)
 
 End abs_history_lemmas.
